StructuredEncryption/src/Paths.dfy
@@ -1,0 +1,286 @@
+// Copyright Amazon.com Inc. or its affiliates. All Rights Reserved.
+// SPDX-License-Identifier: Apache-2.0
+
+include "../Model/AwsCryptographyStructuredEncryptionTypes.dfy"
+
+module Paths {
+  import opened Wrappers
+  import opened StandardLibrary
+  import opened StandardLibrary.UInt
+  import UTF8
+
+  type Bytes = seq<uint8>
+  type GoodString = x : string | ValidString(x)
+  predicate method ValidString(x : string)
+  {
+    && |x| <  UINT64_LIMIT
+    && UTF8.Encode(x).Success?
+  }
+
+  datatype Selector =
+    | List(pos : uint64)
+    | Map(key : GoodString)
+    | Attr(key : GoodString)
+
+  type SelectorList = x : seq<Selector> | |x| < UINT64_LIMIT
+
+  // a specific part of a structure
+  datatype Source = Source (
+    parts : SelectorList
+  )
+  {
+    // Return the Canonical Path for this part of an item in this table
+    function method canonicalPath(table : GoodString)
+      : (ret : Bytes)
+      requires 0 < |parts|
+      ensures ret ==
+          //= specification/structured-encryption/header.md#canoncial-path
+          //= type=implication
+          //# The canoncial path MUST start with the UTF8 encoded table name.
+          UTF8.Encode(table).value
+          //= specification/structured-encryption/header.md#canoncial-path
+          //= type=implication
+          //# This MUST be followed by the depth of the location within a record.
+        + UInt64ToSeq(|parts| as uint64)
+          //= specification/structured-encryption/header.md#canoncial-path
+          //= type=implication
+          //# This MUST be followed by the encoding for each item in the path, including the item itself.
+        + CanonicalPath(parts)
+    {
+      var tableName := UTF8.Encode(table).value;
+      var sourceDepth := UInt64ToSeq(|parts| as uint64);
+      var path := CanonicalPath(parts);
+      tableName + sourceDepth + path
+    }
+  }
+
+  // return the number of characters until the next part begins
+  // that is, '[' or '.'
+  function method  {:opaque} FindStartOfNext(s : string)
+    : (index : Option<nat>)
+    ensures index.Some? ==> 
+      && index.value < |s|
+      && (s[index.value] == '.' || s[index.value] == '[')
+      && '.' !in s[..index.value]
+      && '[' !in s[..index.value]
+    ensures index.None? ==> '.' !in s && '[' !in s
+  {
+    var dot := FindIndexMatching(s, '.', 0);
+    var bracket := FindIndexMatching(s, '[', 0);
+    if dot.None? && bracket.None? then
+      None
+    else if dot.Some? && bracket.Some? then
+      if dot.value < bracket.value then
+        dot
+      else
+        bracket
+    else if dot.Some? then
+      dot
+    else
+      bracket
+  }
+
+  // read an unsigned decomal number, return value and length
+  function method {:tailrecursion} {:opaque} GetNumber(s : string, acc : nat := 0)
+    : Result<nat, string>
+  {
+    if |s| == 0 then
+      Success(acc)
+    else if '0' <= s[0] <= '9' then
+      GetNumber(s[1..], acc * 10 + s[0] as nat - '0' as nat)
+    else
+      Failure("Unexpected character in number : " + [s[0]])
+  }
+
+  // make Map from string
+  function method  {:opaque} MakeMap(s : string) : (ret : Result<Selector, string>)
+    ensures ret.Success? ==> ret.value.Map?
+  {
+    :- Need(ValidString(s), "Key string invalid.");
+    Success(Map(s))
+  }
+
+  // convert string to Selector
+  function method {:opaque} GetSelector(s : string)
+    : Result<Selector, string>
+    requires |s| > 0 && (s[0] == '.' || s[0] == '[')
+  {
+    if s[0] == '.' then
+      var m :- MakeMap(s[1..]);
+      Success(m)
+    else
+      if s[|s|-1] != ']' then
+        Failure("List index must end with ]")
+      else
+        var num :- GetNumber(s[1..|s|-1]);
+        :- Need(num < UINT64_LIMIT, "Array selector exceeds maximum.");
+        Success(List(num as uint64))
+  }
+
+  // convert string to SelectorList
+  function method {:tailrecusrion} {:opaque} GetSelectors(s : string, acc : SelectorList := [])
+    : Result<SelectorList, string>
+    requires |s| > 0 && (s[0] == '.' || s[0] == '[')
+  {
+    var pos := FindStartOfNext(s[1..]);
+    var end := if pos.None? then |s| else pos.value + 1;
+    var sel : Selector :- GetSelector(s[..end]);
+    :- Need(|acc|+1 < UINT64_LIMIT, "Selector Overflow");
+    if pos.None? then
+      Success(acc + [sel])
+    else
+      GetSelectors(s[end..], acc + [sel])
+  }
+
+  // convert string to Source
+  function method {:opaque} MakeSource(s : string)
+    : (ret : Result<Source, string>)
+    ensures ret.Success? ==> 0 < |ret.value.parts|
+  {
+    :- Need(0 < |s|, "Path specification must not be empty.");
+    var pos := FindStartOfNext(s);
+    if pos.None? then
+      var m :- MakeMap(s);
+      Success(Source([m]))
+    else
+      var name := s[..pos.value];
+      var selectors :- GetSelectors(s[pos.value..]);
+      var m :- MakeMap(name);
+      :- Need(|selectors|+1 < UINT64_LIMIT, "Selector Overflow");
+      Success(Source([m] + selectors))
+  }
+
+  // make Source from single top level attribute
+  function method SimpleSource(s : string)
+    : (ret : Result<Source, string>)
+    ensures ret.Success? ==> 0 < |ret.value.parts|
+  {
+    var m :- MakeMap(s);
+    Success(Source([m]))
+  }
+
+  function method SimpleCanon(table : GoodString, attr : GoodString)
+    : Bytes
+  {
+    Source([Map(attr)]).canonicalPath(table)
+  }
+
+  const ARRAY_TAG : uint8 := '#' as uint8
+  const MAP_TAG   : uint8 := '$' as uint8
+  const ATTR_TAG  : uint8 := '@' as uint8
+
+  // get the Canonical Path fragment for this Selector
+  function method CanonicalPart(s : Selector)
+    : (ret : Bytes)
+    //= specification/structured-encryption/header.md#canoncial-path
+    //= type=implication
+    //# object keys in JSON), this MUST be a 0x24 byte ($ in UTF-8),
+    //# followed by the length of the key, followed by the key as a UTF8 string.
+    ensures s.Map? ==> ret == [MAP_TAG] + UInt64ToSeq(|s.key| as uint64) + UTF8.Encode(s.key).value
+    //= specification/structured-encryption/header.md#canoncial-path
+    //= type=implication
+    //# For attributes (XML documents) this MUST be a 0x40 byte (@ in UTF-8),
+    //# followed by the length of the key, followed by the key as a UTF8 string.
+    ensures s.Attr? ==> ret == [ATTR_TAG] + UInt64ToSeq(|s.key| as uint64) + UTF8.Encode(s.key).value
+    //= specification/structured-encryption/header.md#canoncial-path
+    //= type=implication
+    //# For numerical-indexed arrays, this MUST be a 0x23 byte (# in UTF-8), followed by the numerical index.
+    ensures s.List? ==> ret == [ARRAY_TAG] + UInt64ToSeq(s.pos as uint64)
+  {
+    match s {
+      case Map(key) => [MAP_TAG] + UInt64ToSeq(|key| as uint64) + UTF8.Encode(key).value
+      case Attr(key) => [ATTR_TAG] + UInt64ToSeq(|key| as uint64) + UTF8.Encode(key).value
+      case List(pos) => [ARRAY_TAG] + UInt64ToSeq(pos)
+    }
+  }
+
+  // get the Canonical Path for these Selectors
+  function method {:tailrecursion} CanonicalPath(src : SelectorList)
+   : Bytes
+  {
+    if |src| == 0 then
+      []
+    else
+      CanonicalPart(src[0]) + CanonicalPath(src[1..])
+  }
+
+// End code, begin lemmas. 
+// The only useful one is SimpleCanonUnique
+// The others are here to prove that
+
+  lemma CanonicalPartMapUnique(x : Selector, y : Selector)
+    requires x.Map?
+    requires y.Map?
+    requires x != y
+    ensures CanonicalPart(x) != CanonicalPart(y)
+  {
+    assert x.key != y.key;
+    assert CanonicalPart(x) == [MAP_TAG] + UInt64ToSeq(|x.key| as uint64) + UTF8.Encode(x.key).value;
+    assert CanonicalPart(y) == [MAP_TAG] + UInt64ToSeq(|y.key| as uint64) + UTF8.Encode(y.key).value;
+    assert UTF8.Encode(x.key).value != UTF8.Encode(y.key).value;
+    if |x.key| == |y.key| {
+      var prefix := [MAP_TAG] + UInt64ToSeq(|y.key| as uint64);
+      assert CanonicalPart(x) == prefix + UTF8.Encode(x.key).value;
+      assert CanonicalPart(y) == prefix + UTF8.Encode(y.key).value;
+      OnePlusOne(prefix, UTF8.Encode(x.key).value, UTF8.Encode(y.key).value);
+      assert CanonicalPart(x) != CanonicalPart(y);
+    } else {
+      assert UInt64ToSeq(|x.key| as uint64) != UInt64ToSeq(|y.key| as uint64);
+      assert CanonicalPart(x)[1..9] == UInt64ToSeq(|x.key| as uint64);
+      assert CanonicalPart(y)[1..9] == UInt64ToSeq(|y.key| as uint64);
+    }
+  }
+
+  lemma OnePart(src : SelectorList)
+    requires |src| == 1
+    ensures CanonicalPath(src) == CanonicalPart(src[0])
+  {}
+
+  lemma SubstrNE<T>(x : seq<T>, y : seq<T>, len : nat)
+    requires len <= |x|
+    requires len <= |y|
+    requires x[len..] != y[len..]
+    ensures x != y
+  {}
+
+  lemma OnePlusOne<T>(x : seq<T>, y : seq<T>, z : seq<T>)
+    requires y != z
+    ensures x + y != x + z
+  {
+    var newY := x + y;
+    var newZ := x + z;
+    SubstrNE(newY, newZ, |x|);
+  }
+
+  // x != y ==> SimpleCanon(x) != SimpleCanon(y), so we can map with it
+  lemma SimpleCanonUnique2(table : GoodString, x : GoodString, y : GoodString)
+    requires x != y
+    ensures SimpleCanon(table, x) != SimpleCanon(table, y)
+  {
+    assert SimpleCanon(table, x) != SimpleCanon(table, y) by {
+      assert Source([Map(x)]).canonicalPath(table) != Source([Map(y)]).canonicalPath(table) by {
+        OnePart([Map(x)]);
+        OnePart([Map(y)]);
+        CanonicalPartMapUnique(Map(x), Map(y));
+        var prefix := UTF8.Encode(table).value + UInt64ToSeq(1 as uint64);
+        assert Source([Map(x)]).canonicalPath(table) == prefix + CanonicalPart(Map(x));
+        assert Source([Map(y)]).canonicalPath(table) == prefix + CanonicalPart(Map(y));
+        assert CanonicalPart(Map(x)) != CanonicalPart(Map(y));
+        OnePlusOne(prefix, CanonicalPart(Map(x)), CanonicalPart(Map(y)));
+        assert Source([Map(x)]).canonicalPath(table) != Source([Map(y)]).canonicalPath(table);
+      }
+    }
+  }
+
+  // x != y ==> SimpleCanon(x) != SimpleCanon(y), so we can map with it
+  lemma SimpleCanonUnique(table : GoodString)
+    ensures forall x : GoodString, y : GoodString :: x != y ==> SimpleCanon(table, x) != SimpleCanon(table, y)
+  {
+    forall x : GoodString, y : GoodString ensures x != y ==> SimpleCanon(table, x) != SimpleCanon(table, y) {
+      if x != y {
+        SimpleCanonUnique2(table, x, y);
+      }
+    }
+  }
+
+}
